@prefix : <https://w3id.org/ctp#> .
@prefix ns: <http://www.w3.org/2003/06/sw-vocab-status/ns#> .
@prefix ctp: <https://w3id.org/ctp#> .
@prefix org: <http://www.w3.org/ns/org#> .
@prefix owl: <http://www.w3.org/2002/07/owl#> .
@prefix rdf: <http://www.w3.org/1999/02/22-rdf-syntax-ns#> .
@prefix xml: <http://www.w3.org/XML/1998/namespace> .
@prefix xsd: <http://www.w3.org/2001/XMLSchema#> .
@prefix dcam: <http://purl.org/dc/dcam/> .
@prefix foaf: <http://xmlns.com/foaf/0.1/> .
@prefix rdfs: <http://www.w3.org/2000/01/rdf-schema#> .
@prefix skos: <http://www.w3.org/2004/02/skos/core#> .
@prefix vann: <http://purl.org/vocab/vann/> .
@prefix dcterms: <http://purl.org/dc/terms/> .
@prefix powder-s: <http://www.w3.org/2007/05/powder-s#> .
@base <https://w3id.org/ctp#> .

<https://w3id.org/ctp> rdf:type owl:Ontology ;
                        dcterms:abstract """This document describes an ontological module for the creation and structuring of cultural thematic paths, aimed at supporting the linked data publishing and managing for the fruition of cultural heritage.<br>The namespace for CTP terms is <a href=\"https://w3id.org/ctp#\">https://w3id.org/ctp#</a><br> The suggested prefix for CTP namespace is <b>ctp</b>.<br><br>
In this module the following Ontology Design Patterns have been used:<br><ul>
<li> <a href=\"http://www.ontologydesignpatterns.org/cp/owl/list.owl\">http://www.ontologydesignpatterns.org/cp/owl/list.owl</a></li>
<li> <a href=\"http://www.ontologydesignpatterns.org/cp/owl/partof.owl\">http://www.ontologydesignpatterns.org/cp/owl/partof.owl</a></li>
<li> <a href=\"http://www.ontologydesignpatterns.org/cp/owl/place.owl\">http://www.ontologydesignpatterns.org/cp/owl/place.owl</a></li></ul><br>
For more information, consult the <a href=\"https://github.com/TizianaPasciuto/CTP_Ontology/tree/master\">GitHub repository</a><br><br>
This work is developed under the Ph.D. Research Project in Digital Humanities, supported by PON \"Ricerca e Innovazione\" 2014-2020, Asse IV \"Istruzione e ricerca per il recupero\", Azione IV.5 \"Dottorati su tematiche Green\" DM 1061/2021.<br><br>
<img src=\"https://github.com/TizianaPasciuto/CTP_Ontology/blob/master/ConceptualizationCTP_20250109.png?raw=true\" height=\"1000px\" />"""^^rdf:HTML ,
                                         """Questo documento descrive un modulo ontologico per la creazione e la strutturazione di percorsi tematici culturali, mirato a supportare la pubblicazione e la gestione dei dati collegati per la fruizione del patrimonio culturale.<br> Il namespace per i termini CTP è <a href=\"https://w3id.org/ctp#\">https://w3id.org/ctp#</a><br> Il prefisso suggerito per il namespace CTP è <b>ctp</b>.<br><br>
In questo modulo sono stati utilizzati i seguenti Ontology Design Patterns:<br><ul>
<li> <a href=\"http://www.ontologydesignpatterns.org/cp/owl/list.owl\">http://www.ontologydesignpatterns.org/cp/owl/list.owl</a></li>
<li> <a href=\"http://www.ontologydesignpatterns.org/cp/owl/partof.owl\">http://www.ontologydesignpatterns.org/cp/owl/partof.owl</a></li>
<li> <a href=\"http://www.ontologydesignpatterns.org/cp/owl/place.owl\">http://www.ontologydesignpatterns.org/cp/owl/place.owl</a></li></ul><br>
Questo lavoro è stato sviluppato nell'ambito del Progetto di Ricerca per il Dottorato in Discipline Umanistiche Digitali, supportato dal PON \"Ricerca e Innovazione\" 2014-2020, Asse IV \"Istruzione e ricerca per il recupero\", Azione IV.5 \"Dottorati su tematiche Green\" DM 1061/2021.<br>
<img src=\"<img src=\"https://github.com/TizianaPasciuto/CTP_Ontology/blob/master/Conceptualization_TPs_20240306.png?raw=true\" height=\"1000px\" /> -->"""@it ;
                        dcterms:created "2025-01-14"^^xsd:date ;
                        dcterms:creator ctp:atizianapasciuto ,
                                        ctp:briccardoalbertoni ,
                                        ctp:crobertamaggi ;
                        dcterms:license <https://creativecommons.org/licenses/by/4.0/> ;
                        dcterms:title "Cultural Thematic Path (CTP) Ontology"@en ;
                        vann:preferredNamespacePrefix "ctp" ;
                        rdfs:comment """The creation of digital thematic paths represents an innovative approach to the enjoyment of online content, enabling users to navigate in a structured manner through information relevant to a specific topic and/or sector. In order to maximize the effectiveness of such paths, the intention is to develop an ontology that guides in their structure and organization.<br>
The development of an ontology for thematic paths aims not only to provide a clear and comprehensive definition of the concept but also to specify its main and basic requirements and the organization of content. The main purpose is to facilitate the enhancement of cultural heritage by facilitating user navigation through a series of described and interconnected information and resources. This achievement can be attained through the development of an ontology that serves as a tool for the organization, management, exchange, and enjoyment of online information.<br>
With regard to the scope, although the structuring of thematic paths can be related to any sector, in this study the attention will be focused on the GLAM domain. Therefore, the reference scope will be related to the cultural heritage."""^^rdf:HTML ,
                                     """La creazione di percorsi tematici digitali rappresenta un approccio innovativo per la fruizione di contenuti online, consentendo agli utenti di navigare in modo strutturato attraverso informazioni pertinenti a un determinato argomento e/o settore. Al fine di massimizzare l'efficacia di tali percorsi, si intende sviluppare un'ontologia che ne guidi la struttura e l'organizzazione. 
La realizzazione di un'ontologia sui percorsi tematici punta non solo a fornire una definizione chiara ed onnicomprensiva del concetto, ma anche ad esplicitandone i requisiti fondanti e basilari e l'organizzazione dei contenuti. L'obiettivo finale è favorire la valorizzazione del patrimonio culturale, facilitando la navigazione degli utenti attraverso una serie di informazioni e risorse descritte e collegate fra loro. Il suo raggiungimento può essere raggiunto attraverso lo sviluppo di un'ontologia che funga da strumento per l'organizzazione, la gestione, l'interscambio e la fruizione delle informazioni online.
Per quanto riguarda l'ambito, nonostante la strutturazione di percorsi tematici possa essere riferita a qualsiasi settore, in questo studio l'attenzione verrà focalizzata sul dominio GLAM, quindi l'ambito di riferimento sarà circoscritto al patrimonio culturale e la sua valorizzazione."""@it ;
                        rdfs:label "Cultural Thematic Path (CTP) Ontology"@en ;
                        owl:versionInfo "1.0.0" .

#################################################################
#    Annotation properties
#################################################################

###  http://purl.org/dc/terms/abstract
dcterms:abstract rdf:type owl:AnnotationProperty ;
                 rdf:comment "A summary of the resource."@en ;
                 rdfs:comment "A summary of the resource."@en ;
                 rdfs:isDefinedBy dcterms: ;
                 rdfs:label "abstract"@en .


###  http://purl.org/dc/terms/created
dcterms:created rdf:type owl:AnnotationProperty ;
                dcterms:description "Recommended practice is to describe the date, date/time, or period of time as recommended for the property Date, of which this is a subproperty."@en ;
                rdfs:comment "Date of creation of the resource."@en ;
                rdfs:isDefinedBy dcterms: ;
                rdfs:label "dateCreated"@en ;
                rdfs:range rdfs:Literal .


###  http://purl.org/dc/terms/creator
dcterms:creator rdf:type owl:AnnotationProperty ;
                dcterms:description "Recommended practice is to identify the creator with a URI.  If this is not possible or feasible, a literal value that identifies the creator may be provided."@en ;
                rdfs:comment "An entity responsible for making the resource."@en ;
                rdfs:isDefinedBy dcterms: ;
                rdfs:label "creator"@en .


###  http://purl.org/dc/terms/description
dcterms:description rdf:type owl:AnnotationProperty ;
                    dcterms:description "Description may include but is not limited to: an abstract, a table of contents, a graphical representation, or a free-text account of the resource."@en ;
                    rdfs:comment "An account of the resource."@en ;
                    rdfs:isDefinedBy dcterms: ;
                    rdfs:label "description"@en .


###  http://purl.org/dc/terms/identifier
dcterms:identifier rdf:type owl:AnnotationProperty ;
                   dcterms:description "Recommended practice is to identify the resource by means of a string conforming to an identification system. Examples include International Standard Book Number (ISBN), Digital Object Identifier (DOI), and Uniform Resource Name (URN).  Persistent identifiers should be provided as HTTP URIs."@en ;
                   rdfs:comment "An unambiguous reference to the resource within a given context."@en ;
                   rdfs:isDefinedBy dcterms: ;
                   rdfs:label "identifier"@en ;
                   rdfs:range rdfs:Literal .


###  http://purl.org/dc/terms/license
dcterms:license rdf:type owl:AnnotationProperty .


###  http://purl.org/dc/terms/subject
dcterms:subject rdf:type owl:AnnotationProperty ;
                dcterms:description "Recommended practice is to refer to the subject with a URI. If this is not possible or feasible, a literal value that identifies the subject may be provided. Both should preferably refer to a subject in a controlled vocabulary."@en ;
                rdfs:comment "A topic of the resource."@en ;
                rdfs:isDefinedBy dcterms: ;
                rdfs:label "subject"@en .


###  http://purl.org/dc/terms/title
dcterms:title rdf:type owl:AnnotationProperty ;
              rdfs:comment "A name given to the resource."@en ;
              rdfs:isDefinedBy dcterms: ;
              rdfs:label "title"@en ;
              rdfs:range rdfs:Literal .


###  http://purl.org/dc/terms/type
dcterms:type rdf:type owl:AnnotationProperty ;
             dcterms:description "Recommended practice is to use a controlled vocabulary such as the DCMI Type Vocabulary [[DCMI-TYPE](http://dublincore.org/documents/dcmi-type-vocabulary/)]. To describe the file format, physical medium, or dimensions of the resource, use the property Format."@en ;
             rdfs:comment "The nature or genre of the resource."@en ;
             rdfs:isDefinedBy dcterms: ;
             rdfs:label "type"@en .


###  http://purl.org/vocab/vann/example
vann:example rdf:type owl:AnnotationProperty .


###  http://purl.org/vocab/vann/preferredNamespacePrefix
vann:preferredNamespacePrefix rdf:type owl:AnnotationProperty .


###  http://purl.org/vocab/vann/usageNote
vann:usageNote rdf:type owl:AnnotationProperty .


###  http://www.w3.org/1999/02/22-rdf-syntax-ns#comment
rdf:comment rdf:type owl:AnnotationProperty .


###  http://www.w3.org/2003/06/sw-vocab-status/ns#termStatus
ns:termStatus rdf:type owl:AnnotationProperty .


###  http://www.w3.org/2004/02/skos/core#Concept
skos:Concept rdf:type owl:AnnotationProperty .


###  http://www.w3.org/2004/02/skos/core#altLabel
skos:altLabel rdf:type owl:AnnotationProperty .


###  http://www.w3.org/2004/02/skos/core#changeNote
skos:changeNote rdf:type owl:AnnotationProperty .


###  http://www.w3.org/2004/02/skos/core#definition
skos:definition rdf:type owl:AnnotationProperty .


###  http://www.w3.org/2004/02/skos/core#editorialNote
skos:editorialNote rdf:type owl:AnnotationProperty .


###  http://www.w3.org/2004/02/skos/core#scopeNote
skos:scopeNote rdf:type owl:AnnotationProperty .


###  http://www.w3.org/2007/05/powder-s#describedby
powder-s:describedby rdf:type owl:AnnotationProperty .


###  http://www.w3.org/ns/org#memberOf
org:memberOf rdf:type owl:AnnotationProperty .


###  http://xmlns.com/foaf/0.1/homepage
foaf:homepage rdf:type owl:AnnotationProperty .


###  http://xmlns.com/foaf/0.1/name
foaf:name rdf:type owl:AnnotationProperty .


#################################################################
#    Datatypes
#################################################################

###  http://www.w3.org/1999/02/22-rdf-syntax-ns#HTML
rdf:HTML rdf:type rdfs:Datatype .


###  http://www.w3.org/2000/01/rdf-schema#Resource
rdfs:Resource rdf:type rdfs:Datatype .


###  http://www.w3.org/2001/XMLSchema#date
xsd:date rdf:type rdfs:Datatype .


#################################################################
#    Object Properties
#################################################################

###  https://w3id.org/ctp#IsInvolvedIn
ctp:IsInvolvedIn rdf:type owl:ObjectProperty ;
                 owl:inverseOf ctp:involves ;
                 rdfs:domain ctp:Agent ;
                 rdfs:range ctp:RelationToAgent ;
                 rdfs:comment "Indica l'agente coinvolto in una relazione."@it ,
                              "Indicates the agent involved in a relation."@en ;
                 rdfs:label "isInvolvedIn"@en .


###  https://w3id.org/ctp#agentRefersTo
ctp:agentRefersTo rdf:type owl:ObjectProperty ;
                  rdfs:subPropertyOf ctp:isSubjectOf ;
                  owl:inverseOf ctp:refersToAgent ;
                  rdfs:domain ctp:Agent ;
                  rdfs:range ctp:ThematicPath ;
                  rdfs:comment "Indica la relazione fra un agente e un percorso tematico al quale si riferisce."@it ,
                               "Indicates the relationship between an agent and the thematic path to which it refers."@en ;
                  rdfs:label "agentRefersTo"@en .


###  https://w3id.org/ctp#allowsTheSaleOf
ctp:allowsTheSaleOf rdf:type owl:ObjectProperty ;
                    owl:inverseOf ctp:soldThrough ;
                    rdfs:domain ctp:ThematicPath ;
                    rdfs:range ctp:Product ;
                    rdfs:comment "Indica che una risorsa legata a un percorso tematico può essere venduta attraverso il percorso stesso (ad esempio, il catalogo di una mostra descritta dal percorso tematico)."@it ,
                                 "Indicates that a thematic path is linked to a resource that can be sold during its use (e.g. the catalog of an exhibition described by the thematic path)."@en ;
                    rdfs:label "allowsTheSaleOf"@en ;
                    skos:editorialNote "Preferred direction of the relationship."@en .


###  https://w3id.org/ctp#conformsTo
ctp:conformsTo rdf:type owl:ObjectProperty ;
               owl:inverseOf ctp:isConformedBy ;
               rdfs:domain ctp:SecondaryMetadataDescription ;
               rdfs:range ctp:Standard ;
               rdfs:comment "Indica il tipo di standard (CIDOC-CRM, RiC-O, and so on) adoperato nella descrizione dei metadati di una risorsa culturale."@it ,
                            "It indicates the type of standard (CIDOC-CRM, RiC-O, and so on) is used for the metadata description of a cultural resource."@en ;
               rdfs:label "conformsTo"@en ;
               skos:editorialNote "Preferred direction of the relationship."@en .


###  https://w3id.org/ctp#hasBeginning
ctp:hasBeginning rdf:type owl:ObjectProperty ;
                 rdfs:subPropertyOf ctp:hasTime ;
                 owl:inverseOf ctp:isBeginningOf ;
                 rdfs:domain ctp:TemporalEntity ;
                 rdfs:range ctp:Instant ;
                 rdfs:comment "Beginning of a temporal entity."@en ,
                              "Inizio di un'entità temporale."@it ;
                 rdfs:label "hasBeginning"@en ;
                 skos:editorialNote "Preferred direction of the relationship."@en .


###  https://w3id.org/ctp#hasCreator
ctp:hasCreator rdf:type owl:ObjectProperty ;
               owl:inverseOf ctp:isCreatorOf ;
               rdfs:domain ctp:Identifier ;
               rdfs:range ctp:Agent ;
               rdfs:comment "Indica tramite quale agente pubblico o privato è stato creato il codice di identificazione della risorsa culturale."@it ,
                            "Indicates by which public or private agent the identification code of the cultural resource was created."@en ;
               rdfs:label "hasCreator"@en ;
               skos:editorialNote "Preferred direction of the relationship."@en .


###  https://w3id.org/ctp#hasEnd
ctp:hasEnd rdf:type owl:ObjectProperty ;
           rdfs:subPropertyOf ctp:hasTime ;
           owl:inverseOf ctp:isEndOf ;
           rdfs:domain ctp:TemporalEntity ;
           rdfs:range ctp:Instant ;
           rdfs:comment "End of a temporal entity."@en ,
                        "Fine di una entità temporale."@it ;
           rdfs:label "hasEnd"@en ;
           skos:editorialNote "Preferred direction of the relationship."@en .


###  https://w3id.org/ctp#hasGeometry
ctp:hasGeometry rdf:type owl:ObjectProperty ;
                owl:inverseOf ctp:isGeometryOf ;
                rdfs:domain ctp:Place ;
                rdfs:range ctp:Geometry ;
                rdfs:comment "Associa un oggetto spaziale con una geometria corrispondente."@it ,
                             "Associates a spatial thing with a corresponding geometry."@en ;
                rdfs:label "hasGeometry"@en ;
                skos:editorialNote "Preferred direction of the relationship."@en .


###  https://w3id.org/ctp#hasItem
ctp:hasItem rdf:type owl:ObjectProperty ;
            owl:inverseOf ctp:isItemOf ;
            rdfs:domain ctp:OrderedListSlot ;
            rdfs:range ctp:CulturalResource ;
            rdfs:comment "Indica una risorsa culturale in una lista ordinata."@it ,
                         "Indicates a slot cultural resource in an ordered list."@en ;
            rdfs:label "hasItem"@en ;
            skos:editorialNote "Preferred direction of the relationship."@en .


###  https://w3id.org/ctp#hasLocation
ctp:hasLocation rdf:type owl:ObjectProperty ;
                owl:inverseOf ctp:isLocationOf ;
                rdfs:domain owl:Thing ;
                rdfs:range ctp:Place ;
                rdfs:comment "Indica la posizione dell'entità. Nel caso di una CulturalResource, ci si riferisce a risorse immobili (ad esempio, beni paesaggistici, edifici storici, chiese, ecc.)."@it ,
                             "Indicates the location of the entity. In the case of CulturalResource, it's referred to immovable resources (e.g. landscape assets, historical buildings, churches, etc.)."@en ;
                rdfs:label "hasLocation"@en ;
                skos:editorialNote "Preferred direction of the relationship."@en .


###  https://w3id.org/ctp#hasMember
ctp:hasMember rdf:type owl:ObjectProperty ;
              owl:inverseOf ctp:memberOf ;
              rdfs:domain ctp:GroupOfPeople ;
              rdfs:range ctp:Agent ;
              rdfs:comment "Indica che un gruppo (inteso come semplice raggruppamento di persone o come società) ha agenti come membri."@it ,
                           "Indicates that a group (intended as a simple grouping of people or as a company) has agents as members."@en ;
              rdfs:label "hasMember"@en ;
              skos:editorialNote "Preferred direction of the relationship."@en .


###  https://w3id.org/ctp#hasOrderedList
ctp:hasOrderedList rdf:type owl:ObjectProperty ;
                   owl:inverseOf ctp:hasSlot ;
                   rdfs:domain ctp:OrderedListSlot ;
                   rdfs:range ctp:ThematicPath ;
                   rdfs:comment "Indica come sono organizzati gli slot del percorso tematico."@it ,
                                "It indicates how the slots of the thematic path are organized."@en ;
                   rdfs:label "hasOrderedList"@en .


###  https://w3id.org/ctp#hasPart
ctp:hasPart rdf:type owl:ObjectProperty ;
            owl:inverseOf ctp:isPartOf ;
            rdfs:domain ctp:ThematicPath ;
            rdfs:range ctp:CulturalResource ;
            owl:propertyChainAxiom ( ctp:hasSlot
                                     ctp:hasItem
                                   ) ;
            rdfs:comment "Indica la relazione tra il percorso tematico e le risorse culturali che lo compongono."@it ,
                         "Indicates the relationship between the thematic path and the cultural resources that compose it."@en ;
            rdfs:label "hasPart"@en .


###  https://w3id.org/ctp#hasPlace
ctp:hasPlace rdf:type owl:ObjectProperty ;
             owl:inverseOf ctp:isPlaceOf ;
             rdfs:domain ctp:RelationToAgent ;
             rdfs:range ctp:Place ;
             rdfs:comment "Indica la localizzazione di un agente con uno specifico ruolo."@it ,
                          "Indicates the location of an agent with a specific role."@en ;
             rdfs:label "hasPlace"@en ;
             skos:editorialNote "Preferred direction of the relationship."@en .


###  https://w3id.org/ctp#hasRelationToAgent
ctp:hasRelationToAgent rdf:type owl:ObjectProperty ;
                       owl:inverseOf ctp:isRelatedTo ;
                       rdfs:domain owl:Thing ;
                       rdfs:range ctp:RelationToAgent ;
                       rdfs:comment "Indica la relazione tra un'entità e un agente coinvolto con un determinato ruolo."@it ,
                                    "Indicates the relationship between an entity and an agent involved with a certain role."@en ;
                       rdfs:label "hasRelationToAgent"@en ;
                       skos:editorialNote "Preferred direction of the relationship."@en .


###  https://w3id.org/ctp#hasRole
ctp:hasRole rdf:type owl:ObjectProperty ;
            owl:inverseOf ctp:isRoleOf ;
            rdfs:domain ctp:RelationToAgent ;
            rdfs:range ctp:Role ;
            rdfs:comment "Indica il tipo di ruolo svolto dall'agente (ad esempio creatore, finanziatore, ecc.)."@it ,
                         "Indicates the type of role played by the agent (e.g. creator, funder, etc)."@en ;
            rdfs:label "hasRole"@en ;
            skos:editorialNote "Preferred direction of the relationship."@en .


###  https://w3id.org/ctp#hasSecondaryIdentifier
ctp:hasSecondaryIdentifier rdf:type owl:ObjectProperty ;
                           owl:inverseOf ctp:isSecondaryIdentifierOf ;
                           rdfs:domain owl:Thing ;
                           rdfs:range ctp:Identifier ;
                           rdfs:comment "Indica la relazione fra un'entità e il suo codice identificativo."@it ,
                                        "Indicates the relationship beetween an entity and its identification code."@en ;
                           rdfs:label "hasSecondaryIdentifier"@en ;
                           skos:editorialNote "Preferred direction of the relationship."@en .


###  https://w3id.org/ctp#hasSecondaryMetadataDescription
ctp:hasSecondaryMetadataDescription rdf:type owl:ObjectProperty ;
                                    owl:inverseOf ctp:isSecondaryMetadataDescriptionOf ;
                                    rdfs:domain ctp:CulturalResource ;
                                    rdfs:range ctp:SecondaryMetadataDescription ;
                                    rdfs:comment "Questa relazione è adoperata per indicare che una risorsa culturale è stata descritta secondo un determinato standard (RiC-O, CIDOC-CRM, e via dicendo)."@it ,
                                                 "This relation is used to indicated that a cultural resource has been described according to a specific standard (RiC-O, CIDOC-CRM, and so on)."@en ;
                                    rdfs:label "hasSecondaryMetadataDescription"@en ;
                                    skos:editorialNote "Preferred direction of the relationship."@en .


###  https://w3id.org/ctp#hasSlot
ctp:hasSlot rdf:type owl:ObjectProperty ;
            rdfs:domain ctp:ThematicPath ;
            rdfs:range ctp:OrderedListSlot ;
            rdfs:comment "Per consentire la classificazione delle risorse culturali secondo un determinato criterio, il percorso tematico è organizzato attraverso slot che possono essere indicizzati."@it ,
                         "To allow the sorting of cultural resources according to a certain criterion, the thematic path is organized through slots that can be indexed."@en ;
            rdfs:label "hasSlot"@en ;
            skos:editorialNote "Preferred direction of the relationship."@en .


###  https://w3id.org/ctp#hasSubject
ctp:hasSubject rdf:type owl:ObjectProperty ;
               owl:inverseOf ctp:isSubjectOf ;
               rdfs:domain owl:Thing ;
               rdfs:range ctp:Subject ;
               rdfs:comment "Indica a quale/i soggetto/i l'entità si riferisce."@it ,
                            "Indicates to which subject/subjects the entity refers."@en ;
               rdfs:label "hasSubject"@en ;
               skos:editorialNote "Preferred direction of the relationship."@en .


###  https://w3id.org/ctp#hasTheme
ctp:hasTheme rdf:type owl:ObjectProperty ;
             owl:inverseOf ctp:isThemeOf ;
             rdfs:domain ctp:ThematicPath ;
             rdfs:range ctp:Theme ;
             rdfs:comment "Indica che il percorso tematico si basa su un tema."@it ,
                          "Indicates that the thematic path is based on a theme."@en ;
             rdfs:label "hasTheme"@en ;
             skos:editorialNote "Preferred direction of the relationship."@en .


###  https://w3id.org/ctp#hasTime
ctp:hasTime rdf:type owl:ObjectProperty ;
            owl:inverseOf ctp:isTimeOf ;
            rdfs:domain owl:Thing ;
            rdfs:range ctp:TemporalEntity ;
            rdfs:comment "Indica il momento in cui un'entità è stata creata e/o un evento è avvenuto."@it ,
                         "Indicates the time an entity was created and/or an event occurred."@en ;
            rdfs:label "hasTime"@en ;
            skos:editorialNote "Preferred direction of the relationship."@en .


###  https://w3id.org/ctp#hasType
ctp:hasType rdf:type owl:ObjectProperty ;
            owl:inverseOf ctp:isTypeOf ;
            rdfs:domain owl:Thing ;
            rdfs:range ctp:Type ;
            rdfs:comment "Indica il tipo di entità."@it ,
                         "Indicates the type of entity."@en ;
            rdfs:label "hasType"@en ;
            skos:editorialNote "Preferred direction of the relationship."@en .


###  https://w3id.org/ctp#hostsTheCulturalEvent
ctp:hostsTheCulturalEvent rdf:type owl:ObjectProperty ;
                          owl:inverseOf ctp:takesPlaceIn ;
                          rdfs:domain ctp:Place ;
                          rdfs:range ctp:CulturalEvent ;
                          rdfs:comment "Indica la relazione tra un evento culturale e il luogo in cui si svolge."@it ,
                                       "Indicates the relationship between a cultural event and the place where it took place."@en ;
                          rdfs:label "hostsTheCulturalEvent"@en .


###  https://w3id.org/ctp#includes
ctp:includes rdf:type owl:ObjectProperty ;
             owl:inverseOf ctp:isIncludedIn ;
             rdfs:domain ctp:ThematicPath ;
             rdfs:range ctp:ThematicPath ;
             rdfs:comment "Indica che un percorso tematico può includere sottopercorsi tematici. Pertanto, possono essere utilizzati come approfondimento degli argomenti trattati precedentemente."@it ,
                          "Indicates that a thematic path may include sub-thematic paths. Therefore, they can be used as a deepening of the topics dealt with previously."@en ;
             rdfs:label "includes"@en .


###  https://w3id.org/ctp#inspires
ctp:inspires rdf:type owl:ObjectProperty ;
             rdfs:subPropertyOf ctp:agentRefersTo ;
             owl:inverseOf ctp:isInspiredByAgent ;
             rdfs:domain ctp:Agent ;
             rdfs:range ctp:ThematicPath ;
             rdfs:comment "Indica la relazione tra un agente che ispira il percorso tematico e il percorso tematico stesso."@it ,
                          "Indicates the relationship between an agent that inspires a thematic path and the thematic path itself."@en ;
             rdfs:label "inspires"@en .


###  https://w3id.org/ctp#involves
ctp:involves rdf:type owl:ObjectProperty ;
             rdfs:domain ctp:RelationToAgent ;
             rdfs:range ctp:Agent ;
             rdfs:comment "Indica quale agente è coinvolto in una relazione con un certo ruolo."@it ,
                          "Indicates which agent is involved in a relationship with a certain role."@en ;
             rdfs:label "involves"@en ;
             skos:editorialNote "Preferred direction of the relationship."@en .


###  https://w3id.org/ctp#isBeginningOf
ctp:isBeginningOf rdf:type owl:ObjectProperty ;
                  rdfs:subPropertyOf ctp:isTimeOf ;
                  rdfs:domain ctp:Instant ;
                  rdfs:range ctp:TemporalEntity ;
                  rdfs:comment "Indica da quale istante inizia un'entità temporale."@it ,
                               "Indicates from which moment a temporal entity begins."@en ;
                  rdfs:label "isBeginningOf"@en .


###  https://w3id.org/ctp#isConformedBy
ctp:isConformedBy rdf:type owl:ObjectProperty ;
                  rdfs:domain ctp:Standard ;
                  rdfs:range ctp:SecondaryMetadataDescription ;
                  rdfs:comment "Indica che un determinato standard (CIDOC-CRM, RiC-O, eccetera) è conforme a fornire una descrizione di metadati secondari di una risorsa culturale."@it ,
                               "It indicates that a specific type of standard (CIDOC-CRM, RiC-O, and so on) is conformed to provide a secondary metadata description of a cultural resource."@en ;
                  rdfs:label "isConformedBy"@en .


###  https://w3id.org/ctp#isCreatorOf
ctp:isCreatorOf rdf:type owl:ObjectProperty ;
                rdfs:domain ctp:Agent ;
                rdfs:range ctp:Identifier ;
                rdfs:comment "Indica l'agente pubblico o privato che crea il codice identificativo della risorsa culturale."@it ,
                             "Indicates the public or private agent that creates the identification code of the cultural resource."@en ;
                rdfs:label "isCreatorOf"@en .


###  https://w3id.org/ctp#isEndOf
ctp:isEndOf rdf:type owl:ObjectProperty ;
            rdfs:subPropertyOf ctp:isTimeOf ;
            rdfs:domain ctp:Instant ;
            rdfs:range ctp:TemporalEntity ;
            rdfs:comment "Indica da quale istante termina un'entità temporale."@it ,
                         "Indicates from which moment a temporal entity ends."@en ;
            rdfs:label "isEndOf"@en .


###  https://w3id.org/ctp#isGeometryOf
ctp:isGeometryOf rdf:type owl:ObjectProperty ;
                 rdfs:domain ctp:Geometry ;
                 rdfs:range ctp:Place ;
                 rdfs:comment "Associa una geometria a un oggetto spaziale."@it ,
                              "Associates a geometry with a spatial entity."@en ;
                 rdfs:label "isGeometryOf"@en .


###  https://w3id.org/ctp#isIncludedIn
ctp:isIncludedIn rdf:type owl:ObjectProperty ;
                 rdfs:domain ctp:ThematicPath ;
                 rdfs:range ctp:ThematicPath ;
                 rdfs:comment "Indica che un sottopercorso tematico è incluso in un percorso tematico."@it ,
                              "Indicates that a sub-thematic path is included in a thematic path."@en ;
                 rdfs:label "isIncludedIn"@en .


###  https://w3id.org/ctp#isInspiredByAgent
ctp:isInspiredByAgent rdf:type owl:ObjectProperty ;
                      rdfs:subPropertyOf ctp:refersToAgent ;
                      rdfs:domain ctp:ThematicPath ;
                      rdfs:range ctp:Agent ;
                      rdfs:comment "Indica la relazione tra il percorso tematico e l'agente che lo ispira."@it ,
                                   "Indicates the relationship between the thematic path and the agent that inspires it."@en ;
                      rdfs:label "isInspiredByAgent"@en ;
                      skos:editorialNote "Preferred direction of the relationship."@en .


###  https://w3id.org/ctp#isItemOf
ctp:isItemOf rdf:type owl:ObjectProperty ;
             rdfs:domain ctp:CulturalResource ;
             rdfs:range ctp:OrderedListSlot ;
             rdfs:comment "Indica una risorsa culturale in una lista ordinata."@it ,
                          "Indicates a slot cultural resource in an ordered list."@en ;
             rdfs:label "isItemOf"@en .


###  https://w3id.org/ctp#isLocationOf
ctp:isLocationOf rdf:type owl:ObjectProperty ;
                 rdfs:domain ctp:Place ;
                 rdfs:range owl:Thing ;
                 rdfs:comment "Indica l'associazione tra una posizione e l'entità che vi è localizzata."@it ,
                              "Indicates the association between a location and the entity that is located there."@en ;
                 rdfs:label "isLocationOf"@en .


###  https://w3id.org/ctp#isPartOf
ctp:isPartOf rdf:type owl:ObjectProperty ;
             rdfs:domain ctp:CulturalResource ;
             rdfs:range ctp:ThematicPath ;
             rdfs:comment "Indica la relazione tra l'oggetto culturale e il/i percorso/percorsi tematico/i a cui è collegato."@it ,
                          "Indicates the relationship between the cultural object and the thematic path/paths to which it is linked."@en ;
             rdfs:label "isPartOf"@en .


###  https://w3id.org/ctp#isPlaceOf
ctp:isPlaceOf rdf:type owl:ObjectProperty ;
              rdfs:domain ctp:Place ;
              rdfs:range ctp:RelationToAgent ;
              rdfs:comment "Indica la localizzazione di un agente con un ruolo specifico."@it ,
                           "Indicates that an agent with a specific role is located in a place."@en ;
              rdfs:label "isPlaceOf"@en .


###  https://w3id.org/ctp#isRealizedIn
ctp:isRealizedIn rdf:type owl:ObjectProperty ;
                 owl:inverseOf ctp:realizes ;
                 rdfs:domain ctp:ThematicPath ;
                 rdfs:range ctp:CulturalEvent ;
                 rdfs:comment "Indica la relazione tra un percorso tematico e un evento culturale che lo origina (ad esempio, una mostra fisica)."@it ,
                              "Indicates the relationship between a thematic path and a cultural event that originates it (e.g. physical exhibition)."@en ;
                 rdfs:label "isRealizedIn"@en ;
                 skos:editorialNote "Preferred direction of the relationship."@en .


###  https://w3id.org/ctp#isRelatedTo
ctp:isRelatedTo rdf:type owl:ObjectProperty ;
                rdfs:domain ctp:RelationToAgent ;
                rdfs:range owl:Thing ;
                rdfs:comment "Indica la relazione tra un'entità e un agente coinvolto con un determinato ruolo."@it ,
                             "Indicates the relationship between an entity and an agent with a certain role."@en ;
                rdfs:label "isRelatedTo"@en .


###  https://w3id.org/ctp#isRoleOf
ctp:isRoleOf rdf:type owl:ObjectProperty ;
             rdfs:domain ctp:Role ;
             rdfs:range ctp:RelationToAgent ;
             rdfs:comment "Indica il tipo di ruolo svolto dall'agente (ad esempio creatore, finanziatore, ecc.)."@it ,
                          "Indicates the type of role played by the agent (e.g. creator, funder, etc)."@en ;
             rdfs:label "isRoleOf"@en .


###  https://w3id.org/ctp#isSecondaryIdentifierOf
ctp:isSecondaryIdentifierOf rdf:type owl:ObjectProperty ;
                            rdfs:domain ctp:Identifier ;
                            rdfs:range owl:Thing ;
                            rdfs:comment "Indica la relazione fra un'entità e il codice identificativo assegnato ad esso da un agente che lo gestisce."@it ,
                                         "Indicates the relationship between an entity and the identification code assigned to it by an agent that manages it."@en ;
                            rdfs:label "isSecondaryIdentifierOf"@en .


###  https://w3id.org/ctp#isSecondaryMetadataDescriptionOf
ctp:isSecondaryMetadataDescriptionOf rdf:type owl:ObjectProperty ;
                                     rdfs:domain ctp:SecondaryMetadataDescription ;
                                     rdfs:range ctp:CulturalResource ;
                                     rdfs:comment "Questa relazione indica che una descrizione di metadati addizionale, che segue un determinato standard (quali ad esempio RiC-O, CIDOC-CRM, eccetera), è disponibile per caratterizzare la risorsa culturale."@it ,
                                                  "This relation indicates that an additional metadata description, following a specific standard (such as RiC-O, CIDOC-CRM, etc.), is available to characterize the cultural resource."@en ;
                                     rdfs:label "isSecondaryMetadataDescriptionOf"@en .


###  https://w3id.org/ctp#isSubjectOf
ctp:isSubjectOf rdf:type owl:ObjectProperty ;
                rdfs:domain ctp:Subject ;
                rdfs:range owl:Thing ;
                rdfs:comment "Indica a quale/i soggetto/i l'entità si riferisce."@it ,
                             "Indicates to which subject/subjects the entity refers."@en ;
                rdfs:label "isSubjectOf"@en .


###  https://w3id.org/ctp#isThemeOf
ctp:isThemeOf rdf:type owl:ObjectProperty ;
              rdfs:domain ctp:Theme ;
              rdfs:range ctp:ThematicPath ;
              rdfs:comment "Indica il tema su cui si basa il percorso tematico."@it ,
                           "Indicates the theme on which the thematic path is based."@en ;
              rdfs:label "isThemeOf"@en .


###  https://w3id.org/ctp#isTimeOf
ctp:isTimeOf rdf:type owl:ObjectProperty ;
             rdfs:domain ctp:TemporalEntity ;
             rdfs:range owl:Thing ;
             rdfs:comment "Indica il momento in cui un'entità è stata creata e/o un evento è avvenuto."@it ,
                          "Indicates the time an entity was created and/or an event occurred."@en ;
             rdfs:label "isTimeOf"@en .


###  https://w3id.org/ctp#isTypeOf
ctp:isTypeOf rdf:type owl:ObjectProperty ;
             rdfs:domain ctp:Type ;
             rdfs:range owl:Thing ;
             rdfs:comment "Indica di che tipologia è l'entità."@it ,
                          "Indicates what type the entity belongs to."@en ;
             rdfs:label "isTypeOf"@en .


###  https://w3id.org/ctp#memberOf
ctp:memberOf rdf:type owl:ObjectProperty ;
             rdfs:domain ctp:Agent ;
             rdfs:range ctp:GroupOfPeople ;
             rdfs:comment "Indica che un agente fa parte di un gruppo, inteso come semplice raggruppamento di persone o come società."@it ,
                          "Indicates that an agent is part of a group, intended as a simple grouping of people or as a company."@en ;
             rdfs:label "memberOf"@en .


###  https://w3id.org/ctp#nextItem
ctp:nextItem rdf:type owl:ObjectProperty ;
             owl:inverseOf ctp:previousItem ;
             rdfs:domain ctp:OrderedListSlot ;
             rdfs:range ctp:OrderedListSlot ;
             rdfs:comment "In an ordered collection, indicates the link to the next item in a list."@en ,
                          "In un insieme ordinato, indica il collegamento all'elemento successivo in un elenco."@it ;
             rdfs:label "nextItem"@en .


###  https://w3id.org/ctp#placeRefersTo
ctp:placeRefersTo rdf:type owl:ObjectProperty ;
                  rdfs:subPropertyOf ctp:isSubjectOf ;
                  owl:inverseOf ctp:refersToPlace ;
                  rdfs:domain ctp:Place ;
                  rdfs:range ctp:ThematicPath ;
                  rdfs:comment "Indica la relazione tra il percorso tematico e i luoghi a cui è collegato."@it ,
                               "It indicates the relationship between the thematic path and the places to which it is linked."@en ;
                  rdfs:label "placeRefersTo"@en .


###  https://w3id.org/ctp#previousItem
ctp:previousItem rdf:type owl:ObjectProperty ;
                 rdfs:domain ctp:OrderedListSlot ;
                 rdfs:range ctp:OrderedListSlot ;
                 rdfs:comment "In an ordered collection, indicates the link to the previous item in a list."@en ,
                              "In un insieme ordinato, indica il collegamento all'elemento precedente in un elenco."@it ;
                 rdfs:label "previousItem"@en .


###  https://w3id.org/ctp#realizes
ctp:realizes rdf:type owl:ObjectProperty ;
             rdfs:domain ctp:CulturalEvent ;
             rdfs:range ctp:ThematicPath ;
             rdfs:comment "Indica la relazione tra un percorso tematico e un evento culturale che lo origina (ad esempio, una mostra fisica)."@it ,
                          "Indicates the relationship between a thematic path and a cultural event that originates it (e.g. physical exhibition)."@en ;
             rdfs:label "realizes"@en .


###  https://w3id.org/ctp#refersToAgent
ctp:refersToAgent rdf:type owl:ObjectProperty ;
                  rdfs:subPropertyOf ctp:hasSubject ;
                  rdfs:domain ctp:ThematicPath ;
                  rdfs:range ctp:Agent ;
                  rdfs:comment "Indica la relazione fra il percorso tematico e l'agente con il quale è collegato."@it ,
                               "It indicates the relationship between the thematic path and the agent to which is linked."@en ;
                  rdfs:label "refersToAgent"@en ;
                  skos:editorialNote "Preferred direction of the relationship."@en .


###  https://w3id.org/ctp#refersToPlace
ctp:refersToPlace rdf:type owl:ObjectProperty ;
                  rdfs:subPropertyOf ctp:hasSubject ;
                  rdfs:domain ctp:ThematicPath ;
                  rdfs:range ctp:Place ;
                  rdfs:comment "Indica la relazione tra il percorso tematico e i luoghi a cui è collegato."@it ,
                               "It indicates the relationship between the thematic path and the places to which it is linked."@en ;
                  rdfs:label "refersToPlace"@en ;
                  skos:editorialNote "Preferred direction of the relationship."@en .


###  https://w3id.org/ctp#refersToTemporalEntity
ctp:refersToTemporalEntity rdf:type owl:ObjectProperty ;
                           rdfs:subPropertyOf ctp:hasSubject ;
                           owl:inverseOf ctp:temporalEntityRefersTo ;
                           rdfs:domain ctp:ThematicPath ;
                           rdfs:range ctp:TemporalEntity ;
                           rdfs:comment "Indica la relazione tra il percorso tematico e il periodo storico a cui si riferisce."@it ,
                                        "Indicates the relationship between the thematic path and the historical period to which it refers."@en ;
                           rdfs:label "refersToTemporalEntity"@en ;
                           skos:editorialNote "Preferred direction of the relationship."@en .


###  https://w3id.org/ctp#soldThrough
ctp:soldThrough rdf:type owl:ObjectProperty ;
                rdfs:domain ctp:Product ;
                rdfs:range ctp:ThematicPath ;
                rdfs:comment "Indica una risorsa collegata al percorso tematico che può essere venduta durante il suo utilizzo (ad esempio, il catalogo di una mostra descritta dal percorso tematico)."@it ,
                             "Indicates a resource linked to the thematic path that can be sold during its use (e.g. the catalog of an exhibition described by the thematic path)."@en ;
                rdfs:label "soldThrough"@en .


###  https://w3id.org/ctp#takesPlaceIn
ctp:takesPlaceIn rdf:type owl:ObjectProperty ;
                 rdfs:domain ctp:CulturalEvent ;
                 rdfs:range ctp:Place ;
                 rdfs:comment "Indica la relazione tra un evento culturale e il luogo in cui si è svolto."@it ,
                              "Indicates the relationship between a cultural event and the place where it took place."@en ;
                 rdfs:label "takePlaceIn"@en ;
                 skos:editorialNote "Preferred direction of the relationship."@en .


###  https://w3id.org/ctp#temporalEntityRefersTo
ctp:temporalEntityRefersTo rdf:type owl:ObjectProperty ;
                           rdfs:subPropertyOf ctp:isSubjectOf ;
                           rdfs:domain ctp:TemporalEntity ;
                           rdfs:range ctp:ThematicPath ;
                           rdfs:comment "Indica la relazione tra un periodo storico e il percorso tematico al quale è collegato."@it ,
                                        "It indicates the relationship between an historical period and the thematic path to which it is linked."@en ;
                           rdfs:label "temporalEntityRefersTo"@en .


#################################################################
#    Data properties
#################################################################

###  https://w3id.org/ctp#conveys
ctp:conveys rdf:type owl:DatatypeProperty ;
            rdfs:domain ctp:ThematicPath ;
            rdfs:range rdfs:Literal ;
            rdfs:comment "Indica un messaggio che può trasmettere valori culturali, etici e sociali attraverso il percorso tematico."@it ,
                         "Indicates a message that can convey cultural, ethical and social values through the thematic path."@en ;
            rdfs:label "conveys"@en .


###  https://w3id.org/ctp#hasBoundingBox
ctp:hasBoundingBox rdf:type owl:DatatypeProperty ;
                   rdfs:domain ctp:Place ;
                   rdfs:range rdfs:Literal ;
                   rdfs:comment "Il riquadro delimitatore geografico di un oggetto spaziale."@it ,
                                "The geographic bounding box of a spatial thing."@en ;
                   rdfs:label "hasBoundingBox"@en .


###  https://w3id.org/ctp#hasCentroid
ctp:hasCentroid rdf:type owl:DatatypeProperty ;
                rdfs:domain ctp:Place ;
                rdfs:range rdfs:Literal ;
                rdfs:comment "Il centro geografico (centroide) di un oggetto spaziale."@it ,
                             "The geographic center (centroid) of a spatial thing."@en ;
                rdfs:label "hasCentroid"@en .


###  https://w3id.org/ctp#hasCreationDate
ctp:hasCreationDate rdf:type owl:DatatypeProperty ;
                    rdfs:domain ctp:ThematicPath ;
                    rdfs:range xsd:date ;
                    rdfs:comment "Indica quando è stato creato il percorso tematico."@it ,
                                 "Indicates when the thematic path was created."@en ;
                    rdfs:label "hasCreationDate"@en .


###  https://w3id.org/ctp#hasDate
ctp:hasDate rdf:type owl:DatatypeProperty ;
            rdfs:domain ctp:TemporalEntity ;
            rdfs:range xsd:date ;
            rdfs:comment "Indica una data o un intervallo cronologico che caratterizza un'entità."@it ,
                         "Indicates a date or a chronological range that characterizes an entity."@en ;
            rdfs:label "hasDate"@en .


###  https://w3id.org/ctp#hasDescription
ctp:hasDescription rdf:type owl:DatatypeProperty ;
                   rdfs:domain owl:Thing ;
                   rdfs:range rdfs:Literal ;
                   rdfs:comment "Indica una descrizione di un'entità."@it ,
                                "Indicates a description of an entity."@en ;
                   rdfs:label "hasDescription" .


###  https://w3id.org/ctp#hasIndex
ctp:hasIndex rdf:type owl:DatatypeProperty ;
             rdfs:domain ctp:OrderedListSlot ;
             rdfs:range rdfs:Literal ;
             rdfs:comment "Indica come le risorse culturali vengono indicizzate all'interno del percorso tematico, in modo che appaiano ordinate secondo un criterio specifico (ad esempio, alfabetico, cronologico, ecc.)."@it ,
                          "Indicates how cultural resources are indexed within the thematic path, so they appear ordered according to a specific criterion (e.g. alphabetical, chronological, etc)."@en ;
             rdfs:label "hasIndex"@en .


###  https://w3id.org/ctp#hasName
ctp:hasName rdf:type owl:DatatypeProperty ;
            rdfs:domain ctp:Agent ;
            rdfs:range xsd:string ;
            rdfs:comment "Indica il nome associato a un agente."@it ,
                         "Indicates the name associated with an agent."@en ;
            rdfs:label "hasName"@en .


###  https://w3id.org/ctp#hasNotation
ctp:hasNotation rdf:type owl:DatatypeProperty ;
                rdfs:domain ctp:Identifier ;
                rdfs:range rdfs:Literal ;
                rdfs:comment "Indica il codice di identificazione associato all'entità."@it ,
                             "The string that constitutes the entity identifier."@en ;
                rdfs:label "hasNotation"@en .


###  https://w3id.org/ctp#hasPrimaryIdentifier
ctp:hasPrimaryIdentifier rdf:type owl:DatatypeProperty ;
                         rdfs:domain owl:Thing ;
                         rdfs:range rdfs:Literal ;
                         rdfs:comment "Indica un identificatore univoco della risorsa."@it ,
                                      "It indicates a unique identifier of the entity."@en ;
                         rdfs:label "hasPrimaryIdentifier" .


###  https://w3id.org/ctp#hasTitle
ctp:hasTitle rdf:type owl:DatatypeProperty ;
             rdfs:domain owl:Thing ;
             rdfs:range rdfs:Literal ;
             rdfs:comment "Indica il titolo di un'entità."@it ,
                          "Indicates the title of an entity."@en ;
             rdfs:label "hasTitle"@en .


###  https://w3id.org/ctp#landingPage
ctp:landingPage rdf:type owl:DatatypeProperty ;
                rdfs:domain owl:Thing ;
                rdfs:range rdfs:Resource ;
                rdfs:comment "Indica una pagina web a cui si può accedere tramite un browser per visualizzare un catalogo, un dataset, le loro distribuzioni, e/o informazioni relative aggiuntive riguardanti l'entità."@it ,
                             "Indicates a web page that can be accessed in a browser to view a catalog, a dataset, its distributions, and/or additional related information about the entity."@en ;
                rdfs:label "landingPage"@en .


###  https://w3id.org/ctp#linkToDigitalization
ctp:linkToDigitalization rdf:type owl:DatatypeProperty ;
                         rdfs:domain owl:Thing ;
                         rdfs:range rdfs:Resource ;
                         rdfs:comment "Indica il link che permette di visualizzare l'entità disponibile sul web attraverso un iperlink (per esempio IIIF manifest)."@it ,
                                      "Indicates the link that allows viewing the entity available on the web through an hyperlink (e.g. IIIF manifest)."@en ;
                         rdfs:label "linkToDigitalization"@en .


###  https://w3id.org/ctp#linkToResource
ctp:linkToResource rdf:type owl:DatatypeProperty ;
                   rdfs:domain ctp:SecondaryMetadataDescription ;
                   rdfs:range rdfs:Resource ;
                   rdfs:comment "Indica che il record dell'oggetto culturale è descritto secondo lo standard di terzi e collegato attraverso la descrizione dei metadati secondari."@it ,
                                "Indicates the cultural object record described according to third-party standard and linked through the secondary metadata description."@en ;
                   rdfs:label "linkToResource"@en .


#################################################################
#    Classes
#################################################################

###  https://w3id.org/ctp#Agent
ctp:Agent rdf:type owl:Class ;
          rdfs:comment "An agent, that could be a person, family, group or institution."@en ,
                       "Un agente, che può essere una persona, famiglia, gruppo o istituzione."@it ;
          rdfs:label "Agent"@en .


###  https://w3id.org/ctp#CulturalEvent
ctp:CulturalEvent rdf:type owl:Class ;
                  rdfs:comment "A planned or an unplanned cultural situation that includes a number of activities. It occurs in a certain time and space, and may involve agents."@en ,
                               "Una situazione culturale pianificata o non pianificata che comprende una serie di attività. Si verifica in un determinato tempo e spazio e può coinvolgere agenti."@it ;
                  rdfs:label "CulturalEvent"@en .


###  https://w3id.org/ctp#CulturalResource
ctp:CulturalResource rdf:type owl:Class ;
                     rdfs:comment "A tangible or intangible resource, movable or immovable, realized by nature or man-made, that has been identified as possessing artistic, historical, archaeological, or ethno-anthropological significance."@en ,
                                  "Una risorsa tangibile o intangibile, mobile o immobile, realizzata dalla natura o dall'uomo, identificata come possedente significato artistico, storico, archeologico o etno-antropologico."@it ;
                     rdfs:label "CulturalResource"@en .


###  https://w3id.org/ctp#Geometry
ctp:Geometry rdf:type owl:Class ;
             rdfs:comment "L'identificazione di una posizione come punto, linea, poligono, ecc., espressa utilizzando coordinate in un determinato sistema di riferimento cartesiano."@it ,
                          "The identification of a location as a point, line, polygon, etc. expressed using coordinates in some coordinate reference system."@en ;
             rdfs:label "Geometry"@en .


###  https://w3id.org/ctp#Group
ctp:Group rdf:type owl:Class ;
          rdfs:subClassOf ctp:GroupOfPeople ;
          rdfs:comment "A collection of individual agents that can itself act as an agent, capable of performing actions."@en ,
                       "Una collezione di agenti individuali che può a sua volta agire come un agente, capace di compiere azioni."@it ;
          rdfs:label "Group"@en .


###  https://w3id.org/ctp#GroupOfPeople
ctp:GroupOfPeople rdf:type owl:Class ;
                  rdfs:subClassOf ctp:Agent ;
                  rdfs:comment "A collection of individual agents."@en ,
                               "Una collezione di agenti individuali."@it ;
                  rdfs:label "GroupOfPeople"@en .


###  https://w3id.org/ctp#Identifier
ctp:Identifier rdf:type owl:Class ;
               rdfs:comment "A sequence of characters or symbols that serves to uniquely distinguish an entity or object within a specific system or context."@en ,
                            "Una sequenza di caratteri o simboli che serve a distinguere in modo univoco un'entità o un oggetto all'interno di un sistema o contesto specifico."@it ;
               rdfs:label "Identifier"@en .


###  https://w3id.org/ctp#Instant
ctp:Instant rdf:type owl:Class ;
            rdfs:subClassOf ctp:TemporalEntity ;
            rdfs:comment "A temporal entity with zero extent or duration."@en ,
                         "Un'entità temporale con durata o estensione pari a zero."@it ;
            rdfs:label "Instant"@en .


###  https://w3id.org/ctp#Interval
ctp:Interval rdf:type owl:Class ;
             rdfs:subClassOf ctp:TemporalEntity ;
             rdfs:comment "A temporal entity with an extent or duration."@en ,
                          "Un'entità temporale con un'estensione o una durata."@it ;
             rdfs:label "Interval"@en .


###  https://w3id.org/ctp#OrderedListSlot
ctp:OrderedListSlot rdf:type owl:Class ;
                    rdfs:comment "A thematic path is structured as a collector of cultural objects or present with a casual or predetermined order. In the latter case, cultural objects can be sorted according to a certain criterion (e.g. alphabetical, chronological, in order of author, etc.). This class indicates the slot in an ordered list with a fixed index."@en ,
                                 "Un percorso tematico è strutturato come un collezionista di oggetti culturali o presentato con un ordine casuale o predeterminato. In quest'ultimo caso, gli oggetti culturali possono essere ordinati secondo un certo criterio (ad esempio, alfabetico, cronologico, in base all'autore, ecc.). Questa classe indica lo slot in una lista ordinata con un indice fisso."@it ;
                    rdfs:label "OrderedListSlot"@en .


###  https://w3id.org/ctp#Organization
ctp:Organization rdf:type owl:Class ;
                 rdfs:subClassOf ctp:GroupOfPeople ;
                 owl:disjointWith ctp:Person ;
                 rdfs:comment "A specific type of agent that corresponds to social institutions, such as companies and societies."@en ,
                              "Un tipo specifico di agente che corrisponde a istituzioni sociali, come aziende e società."@it ;
                 rdfs:label "Organization"@en .


###  https://w3id.org/ctp#Person
ctp:Person rdf:type owl:Class ;
           rdfs:subClassOf ctp:Agent ;
           rdfs:comment "Human individuals, regardless of whether they are alive, dead, real, or imaginary."@en ,
                        "Individui umani, indipendentemente dal fatto che siano vivi, morti, reali o immaginari."@it ;
           rdfs:label "Person"@en .


###  https://w3id.org/ctp#Place
ctp:Place rdf:type owl:Class ;
          rdfs:comment "Posizione specifica nello spazio fisico; identifica la localizzazione di qualsiasi entità. Può essere un punto preciso nello spazio (ad esempio, coordinate geografiche) o un'area più ampia (ad esempio, regione geografica)."@it ,
                       "Specific position in physical space; identify the localization of any entity. It can be a precise point in space (e.g. geographical coordinates) or a larger area (e.g. geographical region)."@en ;
          rdfs:label "Place"@en .


###  https://w3id.org/ctp#Product
ctp:Product rdf:type owl:Class ;
            rdfs:comment "A tangible good or an intangible service offered on the market to satisfy consumers' needs or desires."@en ,
                         "Un bene tangibile o un servizio intangibile offerto sul mercato per soddisfare i bisogni o desideri dei consumatori."@it ;
            rdfs:label "Product"@en .


###  https://w3id.org/ctp#RelationToAgent
ctp:RelationToAgent rdf:type owl:Class ;
                    rdfs:comment "Class that allows linking another class to an agent playing a specific role."@en ,
                                 "Classe che consente di collegare un'altra classe a un agente che svolge un ruolo specifico."@it ;
                    rdfs:label "RelationToAgent"@en .


###  https://w3id.org/ctp#Role
ctp:Role rdf:type owl:Class ;
         rdfs:comment "Il ruolo svolto da un agente in un contesto specifico. I termini che caratterizzano i ruoli possono essere tratti da tesauri e vocabolari controllati (ad esempio, il Library of Congress Subject Headings (LCSH) e il Getty's Art & Architecture Thesaurus)."@it ,
                      "The role performed by an agent in a specific context. The terms characterizing the roles can be taken from thesauri and controlled vocabularies (e.g. Library of Congress Subject Headings (LCSH) and Getty's Art & Architecture Thesaurus)."@en ;
         rdfs:label "Role"@en .


###  https://w3id.org/ctp#SecondaryMetadataDescription
ctp:SecondaryMetadataDescription rdf:type owl:Class ;
                                 rdfs:comment "L'identificatore secondario originato da altri sistemi di catalogazione e distinto dall'identifcatore primario del catalogo principale di riferimento."@it ,
                                              "The secondary identifier originates from other cataloging systems and is distinct from the primary identifier of the main reference catalog."@en ;
                                 rdfs:label "SecondaryMetadataDescription"@en .


###  https://w3id.org/ctp#Standard
ctp:Standard rdf:type owl:Class ;
             rdfs:comment "Lo standard utilizzato per descrivere un'entità (per esempio CIDOC-CRM, RiC-O, etc.)."@it ,
                          "The standard used for describing an entity (e.g. CIDOC-CRM, RiC-O, etc.)."@en ;
             rdfs:label "Standard"@en .


###  https://w3id.org/ctp#Subject
ctp:Subject rdf:type owl:Class ;
            rdfs:comment "A concept or a series of concepts that concern and describe the thematic path. The terms characterizing the subjects can be taken from thesauri and controlled vocabularies (e.g. Library of Congress Subject Headings (LCSH) and Getty's Art & Architecture Thesaurus)."@en ,
                         "Un concetto o una serie di concetti che riguardano e descrivono il percorso tematico. I termini che caratterizzano gli argomenti possono essere tratti da tesauri e vocabolari controllati (ad esempio, il Library of Congress Subject Headings (LCSH) e il Getty's Art & Architecture Thesaurus)."@it ;
            rdfs:label "Subject"@en .


###  https://w3id.org/ctp#TemporalEntity
ctp:TemporalEntity rdf:type owl:Class ;
                   owl:equivalentClass [ rdf:type owl:Class ;
                                         owl:unionOf ( ctp:Instant
                                                       ctp:Interval
                                                     )
                                       ] ;
                   rdfs:comment "An abstract concept that allows the measurement of events that occur. It is a dimension in which events take place in the present, in the past and in the future."@en ,
                                "Un concetto astratto che consente la misurazione degli eventi che si verificano. È una dimensione in cui gli eventi hanno luogo nel presente, nel passato e nel futuro."@it ;
                   rdfs:label "TemporalEntity"@en .


###  https://w3id.org/ctp#ThematicPath
ctp:ThematicPath rdf:type owl:Class ;
                 rdfs:comment """A thematic path is a tool for the enjoyment of cultural heritage that allows to connect cultural objects of different nature (tangible and intangible) through the identification of common themes. 
The chosen theme, which may concern specific topics, contexts, events, places, historical periods or characters and so on, is expressed synthetically by a title and in-depth with a written descriptive text; they can be further identified through subjects. 
The thematic path could be structured either as a collector of cultural objects, without establishing an order of priority, or present a predetermined order. 
The development and use of this enjoyment strategy can be profitable to convey messages and cultural, ethical and social values."""@en ,
                              "Un percorso tematico è uno strumento per  la valorizzazione del patrimonio culturale che consente di collegare oggetti culturali di diversa natura (tangibili e intangibili) attraverso l'identificazione di temi comuni. Il tema scelto, che può riguardare argomenti specifici, contesti, eventi, luoghi, periodi storici o personaggi e così via, è espresso in modo sintetico da un titolo e approfondito con un testo descrittivo scritto; possono essere ulteriormente identificati attraverso soggettazioni. Il percorso tematico potrebbe essere strutturato sia come un collezionista di oggetti culturali, senza stabilire un ordine di priorità, sia presentare un ordine predefinito. Lo sviluppo e l'uso di questa strategia di valorizzazione possono essere utili per trasmettere messaggi e valori culturali, etici e sociali."@it ;
                 rdfs:label "ThematicPath"@en .


###  https://w3id.org/ctp#Theme
ctp:Theme rdf:type owl:Class ;
          rdfs:comment "Il soggetto generale del percorso tematico fornisce una descrizione approfondita del tema trattato. Può comprendere uno o più concetti interconnessi, fungendo da preziosa risorsa per scopi di indicizzazione."@it ,
                       "The overall subject of the thematic path providing an in-depth description of the treated subject. It may encompass one or multiple interconnected concepts, serving as a valuable resources for indexing purposes."@en ;
          rdfs:label "Theme"@en .


###  https://w3id.org/ctp#Type
ctp:Type rdf:type owl:Class ;
         rdfs:comment "La categorizzazione di cose o entità che sono raggruppate in base a caratteristiche o attributi condivisi. I termini che caratterizzano le tipologie possono essere tratti da tesauri e vocabolari controllati (ad esempio, il Library of Congress Subject Headings (LCSH) e il Getty's Art & Architecture Thesaurus)."@it ,
                      "The categorization of things or entities that are grouped based on shared characteristics or attributes. The terms characterizing the types can be taken from thesauri and controlled vocabularies (e.g. Library of Congress Subject Headings (LCSH) and Getty's Art & Architecture Thesaurus)."@en ;
         rdfs:label "Type"@en .


#################################################################
#    Individuals
#################################################################

###  https://orcid.org/0000-0001-5648-2713
<https://orcid.org/0000-0001-5648-2713> rdf:type owl:NamedIndividual ;
                                        owl:sameAs ctp:briccardoalbertoni .


###  https://w3id.org/ctp#briccardoalbertoni

###  https://orcid.org/0000-0002-2440-2376
<https://orcid.org/0000-0002-2440-2376> rdf:type owl:NamedIndividual ;
                                        owl:sameAs ctp:atizianapasciuto .


###  https://w3id.org/ctp#atizianapasciuto

###  https://w3id.org/ctp
<https://w3id.org/ctp> rdf:type owl:NamedIndividual .


###  https://w3id.org/ctp#atizianapasciuto
ctp:atizianapasciuto rdf:type owl:NamedIndividual ,
                              ctp:Person ;
                     rdfs:label "Tiziana Pasciuto"@en ;
                     org:memberOf ctp:cnrImati ,
                                  ctp:universitaDiGenova ;
                     foaf:homepage <https://orcid.org/0000-0002-2440-2376> ;
                     foaf:name "Tiziana Pasciuto" .


###  https://w3id.org/ctp#briccardoalbertoni
ctp:briccardoalbertoni rdf:type owl:NamedIndividual ,
                                ctp:Person ;
                       rdfs:label "Riccardo Albertoni"@en ;
                       org:memberOf ctp:cnrImati ;
                       foaf:homepage <https://orcid.org/0000-0001-5648-2713> ;
                       foaf:name "Riccardo Albertoni" .


###  https://w3id.org/ctp#cnrImati
ctp:cnrImati rdf:type owl:NamedIndividual ,
                      ctp:Organization ;
             rdfs:label "Istitute for Applied Mathematics and Information Technologies 'Enrico Magenes'"@en ;
             foaf:homepage "https://imati.cnr.it/" ;
             foaf:name "Istitute for Applied Mathematics and Information Technologies 'Enrico Magenes'" .


###  https://w3id.org/ctp#crobertamaggi
ctp:crobertamaggi rdf:type owl:NamedIndividual ,
                           ctp:Person ;
                  rdfs:label "Roberta Maggi"@en ;
                  org:memberOf ctp:cnrImati ;
                  foaf:name "Roberta Maggi" .


###  https://w3id.org/ctp#universitaDiGenova
ctp:universitaDiGenova rdf:type owl:NamedIndividual ,
                                ctp:Organization ;
                       rdfs:label "University of Genoa, Italy"@en ;
                       foaf:homepage "https://unige.it/" ;
                       foaf:name "University of Genoa, Italy" .


###  Generated by the OWL API (version 4.5.26.2023-07-17T20:34:13Z) https://github.com/owlcs/owlapi
